# Saved by TopBraid on Sat Feb 13 20:01:10 GMT 2010
# baseURI: http://reference.data.gov.uk/def/uri-set/
# imports: http://purl.org/net/provenance/ns
# imports: http://purl.org/dc/elements/1.1/
# imports: http://rdfs.org/ns/void
# imports: http://www.w3.org/2004/02/skos/core

@prefix :        <http://reference.data.gov.uk/def/uri-set/> .
@prefix owl:     <http://www.w3.org/2002/07/owl#> .
@prefix rdf:     <http://www.w3.org/1999/02/22-rdf-syntax-ns#> .
@prefix rdfs:    <http://www.w3.org/2000/01/rdf-schema#> .
@prefix skos:    <http://www.w3.org/2004/02/skos/core#> .
@prefix xsd:     <http://www.w3.org/2001/XMLSchema#> .
@prefix void:	<http://rdfs.org/ns/void#> .

:     rdf:type owl:Ontology ;
      owl:imports <http://purl.org/dc/elements/1.1/> , <http://www.w3.org/2004/02/skos/core> , <http://purl.org/net/provenance/ns> , <http://rdfs.org/ns/void> .

:UriSet
      rdf:type rdfs:Class ;
      rdfs:comment "A class for URI Sets (see <http://www.cabinetoffice.gov.uk/cio/chief_technology_officer/public_sector_ia.aspx>)"^^xsd:string ;
      rdfs:label "Uri Set"^^xsd:string ;
      rdfs:subClassOf <http://rdfs.org/ns/void#Dataset> .

:has-member
      rdf:type rdf:Property ;
      rdfs:comment ""^^xsd:string ;
      rdfs:domain :UriSet ;
      rdfs:label "has-member"^^xsd:string ;
      owl:inverseOf :is-memberOf ;
      skos:prefLabel "has-member"^^xsd:string .

:is-memberOf
      rdf:type rdf:Property ;
      rdfs:comment "A property for associating a thing with a URI Set of which it is a member."^^xsd:string ;
      rdfs:label "is-member of"^^xsd:string ;
      rdfs:range :UriSet ;
      owl:inverseOf :has-member ;
      skos:prefLabel "is-member of"^^xsd:string .

:uriSetClass
      rdf:type rdf:Property ;
      rdfs:comment "A property for associating a URI Sets with an OWL or RDFS class with a URI Set."^^xsd:string ;
      rdfs:domain :UriSet ;
      rdfs:label "uri set class"^^xsd:string ;
      rdfs:range rdfs:Class .

:uriSetConceptScheme
      rdf:type rdf:Property ;
      rdfs:comment "A property for associating a SKOS Concept Scheme with a URI Set"^^xsd:string ;
      rdfs:domain :UriSet ;
      rdfs:label "uri set concept"^^xsd:string ;
      rdfs:range
              [ rdf:type owl:Class ;
                owl:unionOf (skos:Concept skos:ConceptScheme)
              ] .
